SimulationDiv.thy
@@ -1,0 +1,288 @@
+theory SimulationDiv
+imports LTSDiv
+begin
+
+section {* Relating LTSes with divergences: simulation *}
+
+subsection {* Basic definitions *}
+
+text {* 
+  We formalize a notion of simulation with divergences on LTSes. This formalization is carried
+  out having in mind its application to the concept of refinement in the B method. In B, when
+  a module $R$ refines a module $A$, a simulation-like relation is established from $R$ to $A$,
+  i.e. every action taken by $R$, in response to an event that is considered acceptable by $A$
+  shall be simulated by a corresponding action in $A$.
+
+  It is called a gluing invariant and must be such that $R$ cannot diverge in situations where
+  $A$ does not diverge. But $R$ may well be more "robust" and not diverge in a state where $A$
+  would diverge. Of course, in that cases, the behavior of $R$ is not constrained. In the case
+  where $A$ does not diverge, then $R$ must exhibit a behavior that corresponds to one of the
+  possible behaviors of $A$.
+
+  A simulation with divergence is a relation @{text "r"} between the states of one LTS
+  and the states of another LTS such that any transition taken by the former, 
+  \emph{on an event that does not cause the latter to diverge}, can be simulated
+  by the latter. 
+
+  We say that an event @{text "e"} is \emph{accepted} in a state @{text "s"} of a LTS if @{text "(s, e)"}
+  does not belong to the divergences of the LTS (not formalized).
+
+*}
+
+text {*
+  The following function @{text "sim_transition"} lifts a relation on states to
+  a relation on transitions: it requires the source and destination states to be
+  related, and the labels to coincide.
+*}
+
+definition sim_transition :: "'st rel \<Rightarrow> ('st, 'ev) Tr rel" where
+  "sim_transition r \<equiv> { (t,t') | t t'. (src t, src t') \<in> r
+                                     \<and> lbl t = lbl t' \<and> (dst t, dst t') \<in> r }"
+
+text {*
+  Notice that this classic notion of transition is symmetric, since it does not consider
+  possible divergences. Next function is an attempt to rephrase the simulation between 
+  transitions taking into account a set of divergences. 
+*}
+
+definition sim_div_transition :: "'st rel \<Rightarrow> ('st * 'ev) set \<Rightarrow> ('st, 'ev) Tr rel" where
+  "sim_div_transition r d \<equiv> 
+    { (tc,ta) | tc ta. 
+      (src tc, src ta) \<in> r \<and> lbl tc = lbl ta \<and>
+      ((src ta, lbl ta) \<in> d \<or> 
+       (src ta, lbl ta) \<notin> d \<and> (dst tc, dst ta) \<in> r) }"
+
+text {*
+  With this definition, if @{text "(sa, e)"} diverges, then any transition from a state 
+  @{text "sc"} related to @{text "sa"} by @{text "r"}, and labeled @{text "e"} is 
+  considered simulated.
+*}
+
+text {* 
+  A relation @{text r} on states induces a simulation relation of LTS @{text l}
+  by LTS @{text "l'"} if both of the following conditions hold:
+  \begin{itemize}
+  \item Every initial state of @{text l} is related, by @{text "r"} to some initial state 
+    of @{text "l'"}.
+  \item For any states @{text "(s,s')"} related by @{text r} and, for any event @{text "e"}
+    accepted by @{text "l'"}, @{text "e"} is also accepted by @{text "l"} and
+    for any @{text "l"}-transition @{text "t"} from @{text s} labelled by @{text "e"}, there 
+    is an @{text "l'"}-transition @{text "t'"} from @{text "s'"}, also labelled by @{text "e"} 
+    that simulates @{text t}.
+  \end{itemize}
+*}
+
+definition simulation :: "'st rel \<Rightarrow> ('st, 'ev) LTSDiv rel" where
+  "simulation r \<equiv> { (l,l') | l l'.
+     (\<forall>s \<in> init l. \<exists>s' \<in> init l'. (s, s') \<in> r)
+   \<and> (\<forall>s s'. (s, s') \<in> r \<longrightarrow>
+        (\<forall>e . 
+          e \<in> div_state l' s' \<or>
+         (e \<notin> div_state l s \<and> 
+              (\<forall>t \<in> trans l. src t = s \<longrightarrow> lbl t = e \<longrightarrow>
+                   (\<exists>t' \<in> trans l'. src t' = s' \<and> lbl t' = e \<and> (t,t') \<in> sim_transition r))))) }"
+
+text {*
+  The definition of simulation with divergences between LTSes can also be phrased using the
+  simulation with divergences on transitions:
+*}
+
+definition simulation_div :: "'st rel \<Rightarrow> ('st, 'ev) LTSDiv rel" where
+  "simulation_div r \<equiv> { (l,l') | l l'.
+     (\<forall>s \<in> init l. \<exists>s' \<in> init l'. (s, s') \<in> r)
+   \<and> (\<forall>s s'. (s, s') \<in> r \<longrightarrow>
+        (\<forall>t \<in> trans l. src t = s \<longrightarrow>
+           (\<exists>t' \<in> trans l'. src t' = s' \<and> lbl t' = lbl t \<and> 
+              (t,t') \<in> sim_div_transition r (divergences l')))) }"
+
+text {* 
+  We say that @{text "l'"} simulates @{text "l"} (through @{text "r"}), or that 
+  @{text "l"} is simulated by @{text "l'"} through @{text "r"}, if there is a 
+  simulation @{text "r"} from @{text "l"} to @{text "l'"}.
+*}
+definition simulated_by (infixl "\<preceq>" 50)
+where "(l \<preceq> l') \<equiv> \<exists>r. (l,l') \<in> simulation r"
+
+(* A lemma that we might want to prove is the containment of the set of diverging events:
+
+l \<preceq> l' \<longrightarrow>
+s \<in> states l \<longrightarrow>
+s' \<in> states l' \<longrightarrow>
+(s, s') \<in> r \<longrightarrow>
+div_state l s \<subseteq> div_state l' s'
+*)
+
+subsection {* Properties *}
+
+text {*
+  Let us verify some basic properties of simulations. First we have that
+  every LTS simulates itself, through a lifting of the identity relation
+  over states.
+*}
+
+lemma simulation_identity : "(Id::('st,'ev) LTSDiv rel) \<subseteq> simulation (Id::'st rel)" 
+  unfolding simulation_def sim_transition_def by auto
+
+text {*
+   Second, we have that the composition of two simulation relations is a simulation relation.
+*}
+
+lemma simulation_composition:
+  assumes "(l, l') \<in> simulation r" and "(l', l'') \<in> simulation r'"
+  shows "(l, l'') \<in> simulation (r O r')"
+using assms unfolding simulation_def
+  using assms unfolding simulation_def sim_transition_def relcomp_unfold
+  by auto (metis+)
+
+text {* 
+  These properties are lifted to the simulates relation over LTS.
+*}
+
+lemma simulated_by_reflexive: "l \<preceq> l" 
+  unfolding simulated_by_def using simulation_identity by blast
+
+lemma simulates_transitive:
+  assumes "l \<preceq> l'" and "l' \<preceq> l''"
+  shows "l \<preceq> l''"
+  using assms unfolding simulated_by_def using simulation_composition by blast
+
+
+subsection {* Simulation and behavior *}
+
+text {*
+  Similarly, a relation @{text r} on states induces a simulation between two runs:
+  corresponding transitions must be related according to @{text r}, lifted to
+  transitions.
+*}
+definition sim_run :: "'st rel \<Rightarrow> ('st, 'ev) Run rel" where
+  "sim_run r \<equiv> {(ts, ts') | ts ts'. 
+                            list_all2 (\<lambda>t t'. (t,t') \<in> sim_transition r) ts ts'}"
+
+(* original definition -- note that the one above is weaker because it does
+   not enforce that the arguments are actually runs; however, it seems more
+   useful to separate the notions of runs and of simulation.
+inductive sim_run :: "'st rel \<Rightarrow> ('st, 'ev) Run \<Rightarrow> ('st, 'ev) Run \<Rightarrow> bool" where
+  "sim_run' r [] []"
+| "sim_transition r t1 t2 \<Longrightarrow> sim_run r [t1] [t2]"
+| "ts1 \<noteq> [] \<and> sim_run r ts1 ts2 \<and> 
+   sim_transition r t1 t2 \<and> dst t1 = src(hd ts1) \<and> dst t2 = src(hd ts2) \<Longrightarrow> 
+   sim_run r (t1 # ts1) (t2 # ts2)"
+*)
+
+text {*
+  If two runs are similar, they have the same length.
+  In particular, one is empty iff the other one is.
+*}
+lemma sim_run_eq_length: "(ts, ts') \<in> sim_run r \<Longrightarrow> length ts = length ts'"
+  unfolding sim_run_def by (auto dest: list_all2_lengthD)
+
+lemma sim_run_empty_iff: "(ts, ts') \<in> sim_run r \<Longrightarrow> (ts = [] \<longleftrightarrow> ts' = [])"
+  by (auto dest: sim_run_eq_length)
+
+lemma sim_run_empty [simp]:
+  "([], ts) \<in> sim_run r = (ts = [])" 
+  "(ts, []) \<in> sim_run r = (ts = [])"
+  unfolding sim_run_def by auto
+
+text {*
+  Two singleton runs are similar if the transitions are related.
+*}
+lemma sim_run_singleton [simp]:
+  "([t], ts) \<in> sim_run r = (\<exists>t'. ts = [t'] \<and> (t,t') \<in> sim_transition r)"
+  "(ts, [t]) \<in> sim_run r = (\<exists>t'. ts = [t'] \<and> (t',t) \<in> sim_transition r)"
+  unfolding sim_run_def by (auto simp: list_all2_Cons1 list_all2_Cons2)
+
+text {*
+  For two similar runs, all transitions at corresponding positions are related.
+  In particular, the last transitions of two similar, non-empty runs are related,
+  as are the last states.
+*}
+lemma sim_run_nth:
+  "(ts, ts') \<in> sim_run r \<Longrightarrow> \<forall>i < length ts. (ts!i, ts'!i) \<in> sim_transition r"
+  by (simp add: sim_run_def list_all2_conv_all_nth)
+ 
+lemma sim_run_last_trans: 
+  "\<lbrakk> (ts, ts') \<in> sim_run r; ts \<noteq> [] \<rbrakk> \<Longrightarrow> (last ts, last ts') \<in> sim_transition r"
+  by (simp add: last_conv_nth sim_run_empty_iff sim_run_eq_length sim_run_nth)
+
+lemma sim_run_last_state: 
+  "\<lbrakk> (ts, ts') \<in> sim_run r; ts \<noteq> [] \<rbrakk> \<Longrightarrow> (dst (last ts), dst(last ts')) \<in> r"
+  by (auto dest: sim_run_last_trans simp: sim_transition_def)
+
+text {*
+  The concatenation of two similar runs is similar.
+*}
+lemma sim_run_append [simp]:
+  assumes "(us,vs) \<in> sim_run r" and "(xs,ys) \<in> sim_run r"
+  shows "(us @ xs, vs @ ys) \<in> sim_run r"
+  using assms unfolding sim_run_def by (auto intro: list_all2_appendI)
+
+text {*
+  As a special case, appending two similar transitions to two similar runs
+  yields again two similar runs.
+*}
+lemma sim_run_append_trans:
+  assumes "(ts, ts') \<in> sim_run r" and "(t, t') \<in> sim_transition r"
+  shows "(ts @ [t], ts' @ [t']) \<in> sim_run r"
+  using assms by simp
+
+text {*
+  We now prove that a simulation between transition systems gives rise to
+  simulations between runs.
+*}
+
+theorem sim_run:
+  assumes 
+    sim: "(l,l') \<in> simulation r" 
+  and 
+    ts: "ts \<in> runs l"
+  and
+    safe: "\<forall> t . t \<in> set ts \<and> t \<notin> div_trans l'"
+  obtains ts' where "ts' \<in> runs l'" "(ts,ts') \<in> sim_run r"
+proof -
+  from ts have "\<exists>ts' \<in> runs l'. (ts, ts') \<in> sim_run r"
+  proof (induct)
+    show "\<exists>ts' \<in> runs l'. ([], ts') \<in> sim_run r" by (auto intro: runs.base)
+  next
+    fix t
+    assume "t \<notin> div_trans l" "src t \<in> init l"
+    with sim obtain t' where
+      "(src t, src t') \<in> r" "src t' \<in> init l'"
+      "t' \<notin> div_trans l'" "(t,t') \<in> sim_transition r"
+      unfolding simulation_def sorry
+    thus "\<exists>ts'\<in>runs l'. ([t], ts') \<in> sim_run r"
+      by (auto intro: runs.start)
+  next
+    fix t ts
+    assume t: "t \<notin> div_trans l" "src t = dst (last ts)"
+       and ts: "ts \<in> runs l" "ts \<noteq> []"
+       and ih: "\<exists>ts'\<in>runs l'. (ts, ts') \<in> sim_run r"
+    from ih obtain ts' where ts': "ts' \<in> runs l'" "(ts,ts') \<in> sim_run r" by blast
+    from ts ts' have "(dst (last ts), dst (last ts')) \<in> r"
+      by (metis sim_run_last_state)
+    with sim t obtain t' where
+      t': "t' \<notin> div_trans l'" "src t' = dst (last ts')" "(t,t') \<in> sim_transition r"
+      unfolding simulation_def sorry
+    from ts ts' have "ts' \<noteq> []" by (simp add: sim_run_empty_iff)
+    with ts' t' have "ts' @ [t'] \<in> runs l'" by (blast intro: runs.step)
+    with ts' t' show "\<exists>ts'\<in>runs l'. (ts @ [t], ts') \<in> sim_run r"
+      sorry
+  qed
+  with that show ?thesis by blast
+qed
+
+lemma sim_traces:
+  assumes sim: "(l,l') \<in> simulation r" and tev: "(t, ev) \<in> trace_div l"
+  shows "\<exists> (t', ev') \<in> trace_div l'. t = t' \<and> ev' \<subseteq> ev"
+sorry
+
+(*
+theorem sim_trace_inclusion: "(l,l') \<in> simulation r \<Longrightarrow> traces l \<subseteq> traces l'"
+  by (blast dest: sim_traces)
+
+corollary simulates_traces: "l \<preceq> l' \<Longrightarrow> traces l \<subseteq> traces l'"
+  unfolding simulates_def by (auto dest: sim_trace_inclusion)
+*)
+
+end
+
